books/kestrel/risc-v/decoding.lisp
@@ -1,0 +1,73 @@
+; RISC-V Library
+;
+; Copyright (C) 2025 Kestrel Institute (http://www.kestrel.edu)
+; Copyright (C) 2025 Kestrel Technology LLC (http://kestreltechnology.com)
+;
+; License: A 3-clause BSD license. See the LICENSE file distributed with ACL2.
+;
+; Author: Alessandro Coglio (www.alessandrocoglio.info)
+
+;;;;;;;;;;;;;;;;;;;;;;;;;;;;;;;;;;;;;;;;;;;;;;;;;;;;;;;;;;;;;;;;;;;;;;;;;;;;;;;;
+
+(in-package "RISCV")
+
+(include-book "encoding")
+
+(local (include-book "kestrel/built-ins/disable" :dir :system))
+(local (acl2::disable-most-builtin-logic-defuns))
+(local (acl2::disable-builtin-rewrite-rules-for-defaults))
+(set-induction-depth-limit 0)
+
+;;;;;;;;;;;;;;;;;;;;;;;;;;;;;;;;;;;;;;;;;;;;;;;;;;;;;;;;;;;;;;;;;;;;;;;;;;;;;;;;
+
+(defxdoc+ decoding
+  :parents (riscv)
+  :short "Decoding of instructions."
+  :long
+  (xdoc::topstring
+   (xdoc::p
+    "Instructions are encoded as specified in [ISA] and [ISAP],
+     and as formalized in @(see encoding).
+     We declaratively define a decoder as non-executable inverse of the encoder;
+     see @(see decoding-executable) for an equivalent executable decoder."))
+  :order-subtopics t
+  :default-parent t)
+
+;;;;;;;;;;;;;;;;;;;;;;;;;;;;;;;;;;;;;;;;;;;;;;;;;;;;;;;;;;;;;;;;;;;;;;;;;;;;;;;;
+
+(define decode ((enc ubyte32p) (feat featp))
+  :returns (instr? instr-optionp)
+  :short "Declarative definition of instruction decoding."
+  :long
+  (xdoc::topstring
+   (xdoc::p
+    "If there is some valid instruction whose encoding is @('enc'),
+     we return one such instruction.
+     We use the witness function of @(tsee encoding-validp) for that.")
+   (xdoc::p
+    "Since @(tsee encode) is injective (as proved elsewhere),
+     there is in fact at most one such instruction.
+     However, this uniqueness is unnecessary for defining the decoder here.")
+   (xdoc::p
+    "The encoder is left inverse of the decoder over valid encodings.
+     This follows from the same property of the witness function
+     of @(tsee encoding-validp), which is proved there."))
+  (if (encoding-validp enc feat)
+      (encoding-valid-witness (ubyte32-fix enc) (feat-fix feat))
+    nil)
+  :hooks (:fix)
+
+  ///
+
+  (defruled encode-of-decode
+    (implies (encoding-validp enc feat)
+             (equal (encode (decode enc feat) feat)
+                    (ubyte32-fix enc)))
+    :use (:instance lemma (enc (ubyte32-fix enc)) (feat (feat-fix feat)))
+    :prep-lemmas
+    ((defruled lemma
+       (implies (and (ubyte32p enc)
+                     (featp feat)
+                     (encoding-validp enc feat))
+                (equal (encode (decode enc feat) feat)
+                       enc))))))
